cedar-lean/Cedar/Thm/TPE/Input.lean
@@ -26,11 +26,6 @@ open Cedar.Spec
 open Cedar.Validation
 open Cedar.Thm
 
-theorem do_eq_ok₂ {res₁ res₂: Except ε PUnit} :
-  (do res₁ ; res₂) = .ok () → res₁ = .ok () ∧ res₂ = .ok ()
-:= by
-  cases res₁ <;> cases res₂ <;> simp
-
 theorem decide_eq_implies_eq {α} [DecidableEq α] {y : α} :
   ∀ x, decide (x = y) → x = y := by
       simp only [decide_eq_true_eq, imp_self, implies_true]
@@ -91,17 +86,18 @@ partial and concrete parts are validated.
 def IsConsistent (req₁ : Request) (es₁ : Entities) (req₂ : PartialRequest) (es₂ : PartialEntities) : Prop :=
   RequestIsConsistent req₁ req₂ ∧ EntitiesAreConsistent es₁ es₂
 
-theorem consistent_checks_ensure_consistency {env : Environment} (req₁ : Request) (es₁ : Entities) (req₂ : PartialRequest) (es₂ : PartialEntities) :
-  isConsistent env req₁ es₁ req₂ es₂ = .ok () → IsConsistent req₁ es₁ req₂ es₂
+theorem consistent_checks_ensure_consistency {schema : Schema} {req₁ : Request} {es₁ : Entities} {req₂ : PartialRequest} {es₂ : PartialEntities} :
+  isValidAndConsistent schema req₁ es₁ req₂ es₂ = .ok () → IsConsistent req₁ es₁ req₂ es₂
 := by
   intro h
-  simp [isConsistent] at h
+  simp [isValidAndConsistent] at h
+  split at h <;> try cases h
   rcases do_eq_ok₂ h with ⟨h₁, h₂⟩
   simp [IsConsistent]
   constructor
   case _ =>
     simp [RequestIsConsistent]
-    simp [isConsistent.requestIsConsistent] at h₁
+    simp [isValidAndConsistent.requestIsConsistent] at h₁
     split at h₁ <;> simp at h₁
     rcases h₁ with ⟨h₁₁, h₁₂, h₁₃, h₁₄⟩
     constructor
@@ -112,9 +108,9 @@ theorem consistent_checks_ensure_consistency {env : Environment} (req₁ : Reque
     exact partial_is_valid_rfl (fun x => decide (x = req₁.resource)) (fun x => x = req₁.resource) req₂.resource.asEntityUID decide_eq_implies_eq h₁₃
     exact partial_is_valid_rfl (fun x => decide (x = req₁.context)) (fun x => x = req₁.context) req₂.context decide_eq_implies_eq h₁₄
   case _ =>
-    simp [isConsistent.entitiesIsConsistent] at h₂
+    simp [isValidAndConsistent.entitiesIsConsistent] at h₂
     split at h₂ <;> simp at h₂
-    simp [isConsistent.entitiesMatch] at h₂
+    simp [isValidAndConsistent.entitiesMatch] at h₂
     simp [EntitiesAreConsistent]
     intro uid data₂ hᵢ
     replace hᵢ := Data.Map.find?_mem_toList hᵢ
@@ -131,28 +127,6 @@ theorem consistent_checks_ensure_consistency {env : Environment} (req₁ : Reque
     constructor
     exact partial_is_valid_rfl (fun x => decide (x = data₁.ancestors)) (fun x => x = data₁.ancestors) data₂.ancestors decide_eq_implies_eq h₂₂
     exact partial_is_valid_rfl (fun x => decide (x = data₁.tags)) (fun x => x = data₁.tags) data₂.tags decide_eq_implies_eq h₂₃
-
-theorem consistent_checks_ensure_match_environment {env : Environment} {req₂ : PartialRequest} {es₂ : PartialEntities} (req₁ : Request) (es₁ : Entities) :
-  isConsistent env req₁ es₁ req₂ es₂ = .ok () → RequestAndEntitiesMatchEnvironment env req₁ es₁
-:= by
-  intro h
-  simp only [isConsistent] at h
-  rcases do_eq_ok₂ h with ⟨h₁, h₂⟩
-  simp only [isConsistent.requestIsConsistent, Bool.or_eq_true, Bool.not_eq_eq_eq_not,
-    Bool.not_true, Bool.and_eq_true, decide_eq_true_eq] at h₁
-  split at h₁ <;> simp at h₁
-  rename_i h₃
-  simp only [not_or, Bool.not_eq_false] at h₃
-  simp [isConsistent.entitiesIsConsistent] at h₂
-  split at h₂ <;> simp at h₂
-  simp only [isConsistent.entitiesMatch, List.all_eq_true, Prod.forall] at h₂
-  rename_i h₄
-  simp at h₄
-  rcases h₄ with ⟨_, h₄⟩
-  simp only [Except.isOk, Except.toBool] at h₄
-  split at h₄ <;> cases h₄
-  rename_i h₄
-  exact request_and_entities_match_env h₃.right h₄
 
 theorem partial_request_matches_environment (env : Environment) (request : PartialRequest) :
   requestIsValid env request → PartialRequestMatchesEnvironment env request
